completed example of interpretation proof

TAL.v
@@ -5,26 +5,13 @@ Require Import Bool Arith Vector Maps.
 (* 10 registers *)
 Definition K := 10.
 Definition registers := total_map nat.
+Definition empty_regs : registers := t_empty 0.
       
 Inductive aexp : Type :=
 | ANum : nat -> aexp
 | AReg : nat -> aexp
 | APlus : aexp -> aexp -> aexp
 | ASub : aexp -> aexp -> aexp.
-
-Inductive instr : Type :=
-| IAss : forall d : nat, (d < K) -> aexp -> instr
-| IAdd : forall d s : nat, (d < K) -> (s < K) -> instr
-| ISub : forall d s : nat, (d < K) -> (s < K) -> instr
-| IIf : forall d : nat, (d < K) -> aexp -> instr
-| ISeq : instr -> instr -> instr
-| IJmp : aexp -> instr.               
-
-Definition heaps := partial_map instr.
-
-(* Machine State *)
-Inductive st : Type :=
-| St : heaps -> registers -> instr -> st.
 
 (*define relations for aeval , ieval*)
 Fixpoint aeval (a : aexp) (R : registers) : nat :=
@@ -35,21 +22,57 @@ Fixpoint aeval (a : aexp) (R : registers) : nat :=
   | ASub a1 a2 => aeval a1 R - aeval a2 R                
   end.
 
+Inductive instr : Type :=
+| IAss : forall d : nat, (d < K) -> aexp -> instr
+| IAdd : forall d s : nat, (d < K) -> (s < K) -> instr
+| ISub : forall d v : nat, (d < K) -> instr
+| IIf : forall d : nat, (d < K) -> aexp -> instr
+| ISeq : instr -> instr -> instr
+| IJmp : aexp -> instr.
+
+(* Unable to use notations as can't construct proof of d < K on the fly :(
+
+Notation "'R(' d ')' '::=' a" :=
+  (IAss d _ (ANum a)) (at level 60).
+Notation "'R(' s ')' '+:=' 'R(' d ')'" :=
+  (IAdd d s _ _) (at level 60).
+Notation "'R(' s ')' '-:=' v" :=
+  (ISub s v _ ) (at level 60).
+Notation "i1 ;; i2" :=
+  (ISeq i1 i2) (at level 80, right associativity).
+Notation "'JIF' 'R(' d ')' v" :=
+  (IIf d _ (ANum v)) (at level 70).
+Notation "'JUMP' v" :=
+  (IJmp (ANum v)) (at level 80).
+
+Check JIF R(1) 2.
+Check R(1) ::= 10.
+Check R(2) +:= R(1).
+Check R(2) -:= 1.
+Check R(2) +:= R(1) ;; R(2) -:= 1.
+Check JUMP 2.
+*)
+
+      
+Definition heaps := partial_map instr.
+Definition empty_heap : heaps := empty.
+
+(* Machine State *)
+Inductive st : Type :=
+| St : heaps -> registers -> instr -> st.
+
+
 Inductive ieval : instr -> st -> st -> Prop :=
 | R_IAss : forall H R I d a1 pf, ieval (IAss d pf a1) (St H R (ISeq (IAss d pf a1) I)) (St H (t_update R (Id d) (aeval a1 R)) I)
 | R_IAdd : forall H R I d s pf1 pf2, ieval (IAdd d s pf1 pf2) (St H R (ISeq (IAdd d s pf1 pf2) I)) (St H (t_update R (Id s) (aeval (AReg d) R + aeval (AReg s) R)) I)
-| R_ISub : forall H R I d s pf1 pf2, ieval (ISub d s pf1 pf2) (St H R (ISeq (ISub d s pf1 pf2) I)) (St H (t_update R (Id s) (aeval (AReg d) R - aeval (ANum s) R)) I)
-| R_IJmp_Succ : forall H R I I' v, H (Id (R (Id v))) = Some I' -> ieval (IJmp (AReg v)) (St H R I) (St H R I')
-| R_IJmp_Fail : forall H R I v, H (Id (R (Id v))) = None -> ieval I (St H R I) (St H R I)
+| R_ISub : forall H R I d v pf1, ieval (ISub d v pf1) (St H R (ISeq (ISub d v pf1) I)) (St H (t_update R (Id d) (aeval (AReg d) R - aeval (ANum v) R)) I)
+| R_IJmp_Succ : forall H R I' v, H (Id v) = Some I' -> ieval (IJmp (ANum v)) (St H R (IJmp (ANum v))) (St H R I')
+| R_IJmp_Fail : forall H R I v, H (Id v) = None -> ieval I (St H R I) (St H R I)
 | R_IIf_EQ : forall H R I I' v r pf, aeval (AReg r) R = 0 -> (H (Id (R (Id v)))) = Some I' -> ieval (IIf r pf (AReg v)) (St H R I) (St H R I')
 | R_IIf_NEQ : forall H R I v r pf, aeval (AReg r) R <> 0 -> ieval (IIf r pf (AReg v)) (St H R (ISeq (IIf r pf (AReg v)) I)) (St H R I)   
 | R_ISeq : forall st st' st'' i1 i2, ieval i1 st st' -> ieval i2 st' st'' -> ieval (ISeq i1 i2) st st''
 | R_IStuck : forall st i, ieval i st st
 .
-
-Definition empty_heap : heaps := empty.
-
-Definition empty_regs : registers := t_empty 0.
 
 Definition threeLEten := (lt_n_S 2 9 (lt_n_S 1 8 (lt_n_S 0 7 (lt_0_Sn 6)))).
 Definition twoLEten :=  (lt_n_S 1 9 (lt_n_S 0 8 (lt_0_Sn 7))).
@@ -57,8 +80,24 @@ Definition oneLEten :=  (lt_n_S 0 9 (lt_0_Sn 8)).
 
 
 
-Definition init_heap := (update (update (update empty_heap (Id 1) (ISeq (IAss 3 threeLEten (ANum 0)) (IJmp (ANum 2)))) (Id 2) (ISeq (IIf 1 oneLEten (ANum 3)) (ISeq (IAdd 2 3 twoLEten threeLEten) (ISeq (ISub 1 1 oneLEten oneLEten) (IJmp (ANum 2))) ))  )  (Id 3) (IJmp (AReg 4)) ).
+Definition init_heap := (update (update (update empty_heap (Id 1) (ISeq (IAss 3 threeLEten (ANum 0)) (IJmp (ANum 2)))) (Id 2) (ISeq (IIf 1 oneLEten (ANum 3)) (ISeq (IAdd 2 3 twoLEten threeLEten) (ISeq (ISub 1 1 oneLEten) (IJmp (ANum 2))) ))  )  (Id 3) (IJmp (AReg 4)) ).
 
-Print init_heap.
+Definition init_regs :=  (t_update (t_update empty_regs (Id 1) 1) (Id 2) 2).
+Definition final_regs := (t_update (t_update (t_update empty_regs (Id 1) 0) (Id 2) 2) (Id 3) 2).
 
-Example ieval_example1 : ieval (IAss 3 threeLEten (ANum 0)) (St init_heap empty_regs I) .
+Eval compute in init_heap (Id 2).
+
+(* find product of numbers stored in R1 and R2, store in R3
+*)
+Example ieval_jmp_example1 : ieval (ISeq (IAss 3 threeLEten (ANum 0)) (IJmp (ANum 2))) (St init_heap init_regs (ISeq (IAss 3 threeLEten (ANum 0)) (IJmp (ANum 2)))) (St init_heap
+                             (t_update init_regs (Id 3) 0)
+                             (ISeq (IIf 1 oneLEten (ANum 3))
+                                   (ISeq (IAdd 2 3 twoLEten threeLEten)
+                                         (ISeq (ISub 1 1 oneLEten) (IJmp (ANum 2)))))).
+Proof.
+  apply R_ISeq with (St init_heap (t_update init_regs (Id 3) 0) (IJmp (ANum 2))).
+  apply R_IAss.
+  apply R_IJmp_Succ.
+  trivial.
+Qed.
+
